src/datastructures/stack.dfy
@@ -14,11 +14,19 @@ class Node<T> {
 class Stack<T> {
     var top: Node?<T>
 
+    predicate Valid() 
+        reads this
+    {
+        top == null <==> sizeHelper(top) == 0
+    }
+
     method push(data: T)
+        requires Valid()
         modifies this
         ensures fresh(top)
         ensures top.data == data
         ensures top.next == old(top)
+        ensures Valid()
     {
         var toAdd := new Node(data);
         toAdd.next := top;
@@ -30,16 +38,20 @@ class Stack<T> {
     } 
 
     method peek() returns (data: T)
+        requires Valid()
         requires top != null
         ensures data == top.data
+        ensures Valid()
     {
         data := top.data;
     }
 
     method pop() returns (popped: T) 
+        requires Valid()
         requires top != null
         modifies this
         ensures top == old(top.next)
+        ensures Valid()
     {
         popped := top.data;
         top := top.next;
@@ -49,8 +61,25 @@ class Stack<T> {
         // top.next := null; // correctly raises a verification error: may update object not in enclosing context's modifies clause
     }
 
+    method size() returns (s: int)
+        requires Valid()
+        ensures s >= 0
+        ensures Valid()
+    {
+        s := sizeHelper(top);
+    }
+
+    // unable to prove termination
+    function method sizeHelper(node: Node?<T>): int
+        ensures sizeHelper(node) >= 0
+    {
+        if node == null then 0 else 1 + sizeHelper(node.next)
+    } 
+
     method isEmpty() returns (isEmpty: bool) 
+        requires Valid()
         ensures top == null <==> isEmpty
+        ensures Valid()
     {
         if top == null {
             isEmpty := true;
